Moved LZ77 files into `lz77/`, removed compilation of VST related files.

lz77/verif_LZC.v
@@ -1,11 +1,42 @@
 Require Import VST.floyd.proofauto.
 Require Import VST.floyd.library.
-Require Import LZC.
-Require Import LZ LZ_Matching LZ_Tokens Utils.
+Require Import LZ LZ_Matching LZ_Tokens Utils LZC.
 Require Import Stdlib.Strings.Byte.
 
 Instance CompSpecs : compspecs. make_compspecs prog. Defined.
 Definition Vprog : varspecs. mk_varspecs prog. Defined.
+
+Fixpoint get_nth (x n : nat) : nat :=
+  match n with
+    | 0%nat => (x mod 128) + 128
+    | S m => get_nth (x / 128) m
+    end.
+
+Fixpoint nat_to_bytes_fixed (i l x : nat) : list nat :=
+  match l with
+    | 0%nat => []
+    | S p => get_nth x i :: (nat_to_bytes_fixed (i + 1) (p) x)
+  end.
+
+Lemma nat_to_bytes_fixed_len : forall l i x,
+  length (nat_to_bytes_fixed i l x) = l.
+Proof.
+  induction l.
+    - intros. simpl. reflexivity.
+    - intros. simpl. rewrite IHl. reflexivity.
+Qed.
+
+Lemma nat_to_bytes_fixed_sn : forall l i x,
+  nat_to_bytes_fixed i (S l) x = nat_to_bytes_fixed i l x ++ [get_nth x (i + l)].
+Proof.
+  induction l.
+    - intros. simpl. assert (i + 0 = i)%nat by lia. rewrite H. reflexivity.
+    - intros. assert ((nat_to_bytes_fixed i (S (S l)) x) = ((get_nth x (i)) :: (nat_to_bytes_fixed (i+1) (S (l)) x))).
+      simpl. reflexivity.
+      rewrite H. rewrite IHl. simpl. assert (i + 1 + l = i + S l)%nat by lia. rewrite H0. reflexivity.
+Qed.
+
+
 
 (* Adapted from: https://github.com/PrincetonUniversity/VST/blob/master/progs/verif_queue.v *)
 Definition surely_malloc_spec :=
@@ -28,8 +59,6 @@ Definition bytes_to_vals (bs : list nat) : list val :=
 
   Definition bytes_to_nat (bs : list byte) : list nat :=
     (map Byte.to_nat (bs)).
-
-  Print Z.
 
 Definition get_nth_spec :=
   DECLARE _get_nth
@@ -57,20 +86,6 @@ Definition encode_length_spec :=
       SEP (mem_mgr gv;
            data_at sh (tarray tuchar 20) ((bytes_to_vals (nat_to_bytes_fixed 0 20 (Z.to_nat len)))) out_).
 
-(* Definition is_equal_spec :=
-  DECLARE _is_equal
-    WITH sh: share, len: Z, out_: val, out: list val, out_len: Z, s: list val, t: list val, gv: globals
-    PRE [ tptr tuchar, tptr tuchar, tulong ]
-      PROP (writable_share sh; 0 <= len <= Int64.max_unsigned; isptr out_;
-            Zlength (nat_to_bytes (Z.to_nat len)) <= out_len; 0 <= out_len; Zlength initial = 20)
-      PARAMS (s_; t_; Vlong (Int64.repr len)) GLOBALS (gv)
-      SEP (mem_mgr gv; data_at sh (tarray tuchar len) s s_; data_sh (tarray tuchar len) t t_)
-    POST [ tvoid ] 
-      PROP ()
-      RETURN ()
-      SEP (mem_mgr gv;
-           data_at sh (tarray tuchar 20) ((bytes_to_vals (nat_to_bytes_fixed 0 20 (Z.to_nat len)))) out_). *)
-
 Definition is_equal_spec :=
   DECLARE _is_equal
     WITH sh1: share, sh2: share, s_ptr: val, t_ptr: val, len: Z, s_vals: list Z, t_vals: list Z
@@ -96,105 +111,12 @@ Definition is_equal_spec :=
         data_at sh1 (tarray tuchar len) (map Vint (map Int.repr s_vals)) s_ptr;
         data_at sh2 (tarray tuchar len) (map Vint (map Int.repr t_vals)) t_ptr
       ).
-(* 
-Definition decode_length_spec :=
-  DECLARE _decode_length
-    WITH sh_in: share, in_: val, in_bytes: list nat, in_len: Z,
-         sh_out: share, out_: val, gv: globals
-    PRE [ tptr tuchar, tulong, tptr tulong ]
-      PROP (readable_share sh_in; writable_share sh_out;
-            0 <= in_len <= 9; (* HERE IS THE ASSUMPTION. *)
-            in_len = Zlength in_bytes)
-      PARAMS (in_; Vlong (Int64.repr in_len); out_) GLOBALS (gv)
-      SEP (mem_mgr gv;
-           data_at sh_in (tarray tuchar in_len) (map Byte.of_nat in_bytes) in_;
-           data_at sh_out tulong (Vlong Int64.zero) out_)
-    POST [ tulong ] EX idx: Z,
-      PROP (idx = Zlength (nat_to_bytes (fst (bytes_to_nat in_bytes))); 0 <= idx <= in_len)
-      RETURN (Vlong (Int64.repr idx))
-      SEP (mem_mgr gv;
-           data_at sh_out tulong (Vlong (Int64.repr (Z.of_nat (fst (bytes_to_nat in_bytes))))) out_). *)
-
-
-(* Definition find_largest_match_spec :=
-  DECLARE _find_largest_match
-    WITH sh: share, in_: val, in_bytes: list byte, in_len: Z,
-         p: Z, len_: val, off_: val, gv: globals
-    PRE [ tptr tuchar, tulong, tulong, tptr tulong, tptr tulong ]
-      PROP (readable_share sh;
-            0 <= p <= in_len;
-            in_len = Zlength in_bytes;
-            in_len <= Int64.max_unsigned)
-      PARAMS (in_; Vlong (Int64.repr in_len); Vlong (Int64.repr p); len_; off_) GLOBALS (gv)
-      SEP (mem_mgr gv; data_at sh (tarray tuchar in_len) (bytes_to_vals in_bytes) in_)
-    POST [ tvoid ]
-      let result := find_largest_match (slice 0 (Z.to_nat p) in_bytes)
-                                       (slice (Z.to_nat p) (length in_bytes) in_bytes) in
-      PROP () RETURN ()
-      SEP (mem_mgr gv;
-           data_at Ews tulong
-             (Vlong (Int64.repr (Z.of_nat
-               (match result with
-                | Some (len, _) => len
-                | None => 0
-                end)))) len_;
-           data_at Ews tulong
-             (Vlong (Int64.repr (Z.of_nat
-               (match result with
-                | Some (_, off) => off
-                | None => 0
-                end)))) off_). *)
-
-
-Definition compress_out_size (in_len : Z) : Z :=
-  (9 * in_len + 7) / 8 + 65.
-
-(* 
-Definition compress_spec :=
-  DECLARE _compress
-    WITH sh: share, in_: val, in_bytes: list nat, in_len: Z, gv: globals
-    PRE [ tptr tuchar, tulong ]
-      PROP (readable_share sh;
-            0 <= in_len <= Int64.max_unsigned;
-            in_len = Zlength in_bytes)
-      PARAMS (in_; Vlong (Int64.repr in_len)) GLOBALS (gv)
-      SEP (mem_mgr gv; data_at sh (tarray tuchar in_len) (bytes_to_vals in_bytes) in_)
-    POST [ tptr tuchar ] EX p: val,
-      let out_bytes := compress_to_bytes (bytes_to_vals in_bytes) in
-      PROP (Zlength out_bytes <= compress_out_size in_len)
-      RETURN (p)
-      SEP (mem_mgr gv;
-           malloc_token Ews (tarray tuchar (compress_out_size in_len)) p *
-           data_at Ews (tarray tuchar (Zlength out_bytes)) (bytes_to_vals out_bytes) p). *)
-
-(* Definition decompress_spec :=
-  DECLARE _decompress
-    WITH sh: share, in_: val, in_bytes: list byte, in_len: Z, gv: globals
-    PRE [ tptr tuchar, tulong ]
-      PROP (readable_share sh;
-            0 <= in_len <= Int64.max_unsigned;
-            in_len = Z.of_nat (length in_bytes);
-            exists src : list byte,
-              in_bytes = compress_to_bytes src /\ Zlength src <= Int64.max_unsigned)
-      PARAMS (in_; Vlong (Int64.repr in_len)) GLOBALS (gv)
-      SEP (mem_mgr gv; data_at sh (tarray tuchar in_len) (bytes_to_vals in_bytes) in_)
-    POST [ tptr tuchar ] EX p: val,
-      let out_bytes := decompress_from_bytes in_bytes in
-      PROP ()
-      RETURN (p)
-      SEP (mem_mgr gv;
-           data_at sh (tarray tuchar in_len) (bytes_to_vals in_bytes) in_;
-           malloc_token Ews (tarray tuchar (Zlength out_bytes)) p *
-           data_at Ews (tarray tuchar (Zlength out_bytes)) (bytes_to_vals out_bytes) p).
- *)
 
 Definition Gprog: funspecs :=
         ltac:(with_library prog [surely_malloc_spec;
                                  get_nth_spec;
                                  encode_length_spec;
-                                 is_equal_spec
-                                 (* find_largest_match_spec *)
-                                 ]).
+                                 is_equal_spec]).
 
 
 (* Adapted from: https://github.com/PrincetonUniversity/VST/blob/master/progs/verif_queue.v *)
@@ -820,57 +742,4 @@ Proof.
   simpl in H_align.
   Search align_compatible_rec.
 Admitted.
-                  
-(* Lemma decode_length_body:
-  semax_body Vprog Gprog f_decode_length decode_length_spec.
-Proof.
-  start_function.
-  forward_if.
-  - forward.
-    forward.
-    assert (Zlength in_bytes = 0). {
-      assert (Int64.unsigned (Int64.repr (Zlength in_bytes)) = (Zlength in_bytes)). {
-        rewrite Int64.unsigned_repr_eq.
-        rewrite Z.mod_small; [reflexivity | rep_lia].
-      }
-      rewrite H1 in H6.
-      auto.
-    }
-    assert (in_bytes = []) by now apply Zlength_nil_inv.
-    unfold nat_to_bytes.
-    subst. simpl.
-    Exists 0.
-    entailer!!.
-    rewrite H6. 
-    unfold bytes_to_vals. simpl.
-    rewrite data_at_tuchar_zero_array_eq; auto.
-  - forward.
-    (* forward_while ??? *)
-Admitted.
 
-
-Lemma find_largest_match_body: 
-  semax_body Vprog Gprog f_find_largest_match find_largest_match_spec.
-Proof.
-  start_function.
-  forward. forward. forward.
-  (* forward_if ??? *)
-Admitted.
-
-
-Lemma compress_body:
-  semax_body Vprog Gprog f_compress compress_spec.
-Proof.
-  start_function.
-  forward.
-  (* forward_call ??? *)
-Admitted.
-
-Lemma decompress_body:
-  semax_body Vprog Gprog f_decompress decompress_spec.
-Proof.
-  start_function.
-  forward.
-  (* forward_call ??? *)
-Admitted.
- *)
