lz77/LZ_Tokens.v
@@ -1,0 +1,813 @@
+From Stdlib Require Import Arith Strings.Byte List Lia.
+Import ListNotations.
+
+Module Tokens.
+
+  Inductive Token :=
+    | Lit (b: byte)
+    | Ref (length offset: nat). (* 4bit length, 12bit offset *)
+    (*| Ref : forall length offset, 3 <= length <= 18 /\ 3 <= offset <= 4098 -> Token.*)
+
+  Definition valid_token (t: Token) :=
+    match t with
+    | Lit _ => True
+    | Ref length offset => (3 <= length <= 18) /\ (3 <= offset <= 4098)
+    end.
+
+  Section NatBytes.
+
+    Definition nat_to_byte (n: nat): byte :=
+      match of_nat (n mod 256) with
+      | Some b => b
+      | None => x00 (* Never happens *)
+      end.
+
+    Fixpoint nat_to_bytes_fueled (fuel n: nat): list byte :=
+      match fuel with
+      | 0 => []
+      | S fuel =>
+          if n <? 128 then [nat_to_byte n]
+          else let byte := nat_to_byte ((n mod 128) + 128) in
+               byte :: nat_to_bytes_fueled fuel (n / 128)
+      end.
+
+    Definition nat_to_bytes (n: nat): list byte :=
+      nat_to_bytes_fueled n n.
+
+    Fixpoint bytes_to_nat (l: list byte): nat * list byte :=
+      match l with
+      | [] => (0, [])
+      | byte :: tl =>
+          let n := to_nat byte in
+          if n <? 128 then (n, tl)
+          else let (n', tail) := bytes_to_nat tl in
+               ((n mod 128) + 128 * n', tail)
+      end.
+
+    Definition nibbles_to_byte (h l: nat): byte :=
+      nat_to_byte ((h mod 16) * 16 + (l mod 16)).
+
+
+    Lemma nat_to_byte_correctness : forall n,
+      n < 256 ->
+      to_nat (nat_to_byte n) = n.
+    Proof.
+      unfold nat_to_byte.
+      intros.
+      destruct (of_nat (_ mod 256)) eqn:?.
+      - apply to_of_nat_iff.
+        rewrite (Nat.mod_small n 256 ltac:(lia)) in Heqo.
+        assumption.
+      - exfalso.
+        apply of_nat_None_iff in Heqo.
+        pose proof (Nat.mod_upper_bound n 256 ltac:(lia)).
+        lia.
+    Qed.
+
+    Lemma nat_to_bytes_correctness': forall n fuel rest,
+      n <> 0 ->
+      n <= fuel ->
+      bytes_to_nat (nat_to_bytes_fueled fuel n ++ rest) = (n, rest).
+    Proof.
+      induction n as [n IHn] using lt_wf_rec; intros.
+      destruct fuel.
+      - lia.
+      - simpl.
+        destruct (n <? 128) eqn:?; subst; simpl.
+        + apply Nat.ltb_lt in Heqb as Hnl.
+          rewrite nat_to_byte_correctness by lia.
+          rewrite Heqb. reflexivity.
+        + apply Nat.ltb_ge in Heqb as Hng.
+          set (b := nat_to_byte (n mod 128 + 128)).
+          assert (to_nat b = n mod 128 + 128). {
+            apply nat_to_byte_correctness.
+            pose proof (Nat.mod_upper_bound n 128 ltac:(lia)).
+            lia.
+          }
+          match goal with
+          | [ |- context[if to_nat (nat_to_byte ?m) <? _ then _ else _] ] =>
+              assert (Hm: m = n mod 128 + 128) by reflexivity; rewrite Hm; clear Hm
+          end.
+          assert (Heqby: n mod 128 + 128 < 256). {
+            pose proof (Nat.mod_upper_bound n 128 ltac:(lia)). lia.
+          }
+          rewrite nat_to_byte_correctness by lia.
+          assert (Hf: n mod 128 + 128 <? 128 = false). {
+            apply Nat.ltb_ge. lia.
+          }
+          rewrite Hf.
+          replace (fst (Nat.divmod n 127 0 127)) with (n / 128) by reflexivity.
+          assert (Hdiv : n / 128 < n) by (apply Nat.div_lt; lia).
+          assert (n / 128 <> 0). {
+            pose proof (Nat.divmod_spec n 127 0 127 ltac:(lia)).
+            simpl. destruct (Nat.divmod n 127 0 127).
+            simpl. lia.
+          }
+          rewrite (IHn (n / 128) Hdiv fuel rest H2 ltac:(lia)).
+          f_equal.
+          pose proof (Nat.divmod_spec (n mod 128 + 128) 127 0 127 ltac:(lia)).
+          destruct (Nat.divmod (n mod 128 + 128) 127 0 127) as [q u].
+          simpl.
+          match goal with
+          | [ |- ?l + ?r = _ ] =>
+              assert (Hl: l = 127 - u) by reflexivity;
+              assert (Hr: r = 128 * (n / 128)) by reflexivity;
+              rewrite Hl, Hr; clear Hl Hr
+          end.
+          pose proof (Nat.div_mod n 128 ltac:(lia)).
+          lia.
+    Qed.
+
+    Lemma nat_to_bytes_correctness: forall n rest,
+      n <> 0 ->
+      bytes_to_nat (nat_to_bytes n ++ rest) = (n, rest).
+    Proof.
+      intros. unfold nat_to_bytes.
+      rewrite nat_to_bytes_correctness'; auto.
+    Qed.
+
+    Lemma nat_to_bytes_length': forall n fuel,
+      length (nat_to_bytes_fueled fuel n) <= Nat.log2 n / 7 + 1.
+    Proof.
+      induction n as [n IHn] using lt_wf_rec; intros.
+      destruct n, fuel; simpl; try lia.
+      destruct (S n <? 128) eqn:?; simpl; try lia.
+      apply Nat.ltb_ge in Heqb.
+      set (lhs := S (length (nat_to_bytes_fueled fuel (S n / 128)))).
+      set (rhs := Nat.log2 (S n) / 7 + 1).
+      match goal with
+      | [ |- ?l <= ?r ] =>
+          assert (Heq: l = lhs) by reflexivity; rewrite Heq; clear Heq;
+          assert (Heq: r = rhs) by reflexivity; rewrite Heq; clear Heq
+      end.
+      assert (Hdiv: S n / 128 < S n) by (apply Nat.div_lt; lia).
+      assert (Hlog: Nat.log2 (S n / 128) = Nat.log2 (S n) - 7). {
+        destruct n.
+        - simpl. lia.
+        - assert (128 = 2 ^ 7) by reflexivity.
+          rewrite H, <- Nat.shiftr_div_pow2, Nat.log2_shiftr.
+          reflexivity.
+      }
+      specialize (IHn (S n / 128) Hdiv fuel).
+      assert (Hm: lhs <= Nat.log2 (S n / 128) / 7 + 1 + 1) by lia.
+      rewrite Hlog in *.
+
+      etransitivity.
+      - exact Hm.
+      - apply Nat.add_le_mono_r.
+        set (m := Nat.log2 (S n)).
+        assert (7 <= m). {
+          assert (Nat.log2 128 <= m) by now apply Nat.log2_le_mono.
+          unfold Nat.log2 in H.
+          now simpl in H.
+        }
+        simpl.
+        pose proof (Nat.divmod_spec (m - 7) 6 0 6 ltac:(lia)).
+        destruct (Nat.divmod (m - 7) 6 0 6) as [q u].
+        pose proof (Nat.divmod_spec m 6 0 6 ltac:(lia)).
+        destruct (Nat.divmod m 6 0 6) as [q' u'].
+        simpl. lia.
+    Qed.
+
+    Lemma nat_to_bytes_length: forall n,
+      length (nat_to_bytes n) <= Nat.log2 n / 7 + 1.
+    Proof. intro n. exact (nat_to_bytes_length' n n). Qed.
+
+    Lemma to_nat_nibbles_correct : forall h l,
+      h < 16 ->
+      l < 16 ->
+      to_nat (nibbles_to_byte h l) = h * 16 + l.
+    Proof.
+      unfold nibbles_to_byte, nat_to_byte.
+      intros.
+      destruct (of_nat (_ mod 256)) eqn:?.
+      - apply to_of_nat_iff in Heqo.
+        rewrite Heqo.
+        rewrite (Nat.mod_small h 16 ltac:(lia)).
+        rewrite (Nat.mod_small l 16 ltac:(lia)).
+        exact (Nat.mod_small (h * 16 + l) 256 ltac:(lia)).
+      - exfalso.
+        apply of_nat_None_iff in Heqo.
+        pose proof (Nat.mod_upper_bound (h mod 16 * 16 + l mod 16) 256).
+        lia.
+    Qed.
+
+  End NatBytes.
+
+
+
+  Section TokenBytes.
+    Definition token_to_bytes (t: Token): list byte :=
+      match t with
+      | Lit b => [b]
+      | Ref length offset =>
+          let len_opt := length - 3 in
+          let off_opt := offset - 3 in
+          let b0 := nibbles_to_byte len_opt (off_opt / 256) in
+          let b1 := nat_to_byte (off_opt mod 256) in
+          [b0; b1]
+      end.
+
+    Fixpoint tokens_to_bytes_chunk_len (n: nat) (ts: list Token) :=
+      match n, ts with
+      | 0, _ => 0
+      | S pn, [] => 0
+      | S pn, t :: tl => (tokens_to_bytes_chunk_len pn tl) + (length (token_to_bytes t))
+      end.
+
+    Fixpoint tokens_to_bytes_chunk (n: nat) (ts: list Token) :=
+      match n, ts with
+      | 0, _ => ([], ts, [])
+      | S pn, [] => ([], [], [])
+      | S pn, t :: tl =>
+          let flag' := match t with
+                       | Lit _ => true
+                       | Ref _ _ => false end
+          in let '(flag, ts'', acc) :=  tokens_to_bytes_chunk pn tl
+          in (flag' :: flag, ts'', token_to_bytes t ++ acc)
+      end.
+
+    Fixpoint list_bool_to_byte (l: list bool) (x: nat) (n: nat) : byte :=
+      match l, n with
+      | b :: tl, S n => list_bool_to_byte tl (x * 2 + (if b then 1 else 0)) n
+      | _, n => nat_to_byte (x * 2 ^ n)
+      end.
+
+    Fixpoint tokens_to_bytes_fueled (tokens: list Token) (fuel: nat): list byte :=
+      match fuel, tokens with
+      | 0, _ => [] (* Never happens if fuel = length tokens *)
+      | _, [] => []
+      | S fuel, _ =>
+          let '(flag, tail, acc) := tokens_to_bytes_chunk 8 tokens in
+          list_bool_to_byte flag 0 8 :: acc ++ tokens_to_bytes_fueled tail fuel
+      end.
+
+    Definition tokens_to_bytes tokens := tokens_to_bytes_fueled tokens (length tokens).
+
+    Example tokens_to_bytes_test1 :
+      tokens_to_bytes [Lit "000"; Lit "001"; Lit "002"; Lit "003"; Lit "004"; Ref 5 1000] =
+      (* 0b1111_1000 = 248, (2 << 12) + 997 = 9189 = <35, 229> *)
+      ["248"%byte; "000"%byte; "001"%byte; "002"%byte; "003"%byte; "004"%byte; "035"%byte; "229"%byte ].
+    Proof. reflexivity. Qed.
+
+    Example tokens_to_bytes_test2 :
+      tokens_to_bytes [Lit "000"; Lit "001"; Lit "002"; Lit "003"; Lit "004";
+      Lit "005"; Lit "006"; Lit "007"; Lit "008"; Lit "009"; Ref 5 1000] =
+      (* 0b1111_1111 = 255 *)
+      ["255"%byte; "000"%byte; "001"%byte; "002"%byte; "003"%byte; "004"%byte; "005"%byte; "006"%byte; "007"%byte;
+      (* 0b1100_0000 = 192, (2 << 12) + 997 = 9189 = <35, 229> *)
+      "192"%byte; "008"%byte; "009"%byte; "035"%byte; "229"%byte ].
+    Proof. reflexivity. Qed.
+
+    Definition bytes_to_token (l: list byte) (flag: bool): option Token * list byte :=
+      match flag, l with
+      | true, b :: tl => (Some (Lit b), tl)
+      | false, b0 :: b1 :: tl =>
+          let n0 := to_nat b0 in
+          let n1 := to_nat b1 in
+          let len_opt := n0 / 16 in
+          let off_hi := n0 mod 16 in
+          let off_lo := n1 in
+          (Some (Ref (len_opt + 3) (off_hi * 256 + off_lo + 3)), tl)
+      | _, _ => (None, []) (* This may happen if we consumed all bytes but flag had extra bits *)
+      end.
+
+    Fixpoint bytes_to_tokens_chunk (n flag: nat) (after: list byte) : (list Token * list byte) :=
+      match n with
+      | 0 => ([], after)
+      | S pn =>
+          let (otoken, tail) := bytes_to_token after (Nat.testbit flag pn) in
+          match otoken with
+          | Some token =>
+              let (tokens, rest) := bytes_to_tokens_chunk pn flag tail in
+              (token :: tokens, rest)
+          | None => ([], [])
+          end
+      end.
+
+    Fixpoint bytes_to_tokens_fueled (l: list byte) (fuel: nat) : list Token :=
+      match fuel, l with
+      | 0, _ => [] (* Never happens if fuel = length l *)
+      | _, [] => []
+      | S fuel, flag_byte :: tl =>
+          let flag := to_nat flag_byte in
+          let (tokens, tail) := bytes_to_tokens_chunk 8 flag tl
+          in tokens ++ bytes_to_tokens_fueled tail fuel
+      end.
+
+    Definition bytes_to_tokens (l: list byte) : list Token :=
+      bytes_to_tokens_fueled l (length l).
+
+    Example bytes_to_tokens_test1 :
+      bytes_to_tokens ["248"%byte; "000"%byte; "001"%byte; "002"%byte; "003"%byte; "004"%byte; "035"%byte; "229"%byte ] =
+      [Lit "000"; Lit "001"; Lit "002"; Lit "003"; Lit "004"; Ref 5 1000].
+    Proof. reflexivity. Qed.
+
+    Example bytes_to_tokens_test2 :
+      bytes_to_tokens ["255"%byte; "000"%byte; "001"%byte; "002"%byte; "003"%byte; "004"%byte; "005"%byte; "006"%byte; "007"%byte;
+      "192"%byte; "008"%byte; "009"%byte; "035"%byte; "229"%byte ] =
+      [Lit "000"; Lit "001"; Lit "002"; Lit "003"; Lit "004";
+      Lit "005"; Lit "006"; Lit "007"; Lit "008"; Lit "009"; Ref 5 1000].
+    Proof. reflexivity. Qed.
+
+
+    Lemma tokens_to_bytes_chunk_len_correctness: forall n ts flag_byte tail acc,
+      tokens_to_bytes_chunk n ts = (flag_byte, tail, acc) ->
+      tokens_to_bytes_chunk_len n ts = length acc.
+    Proof.
+      induction n; simpl; intros.
+      - inversion H. now simpl.
+      - destruct ts.
+        + inversion H. now simpl.
+        + destruct (tokens_to_bytes_chunk n ts) as [[flag tail'] acc'] eqn:?.
+          rewrite (IHn ts flag tail' acc' Heqp).
+          assert (token_to_bytes t ++ acc' = acc) by congruence.
+          rewrite <- H0, length_app.
+          lia.
+    Qed.
+
+    Lemma to_token_correctness: forall t rest,
+      valid_token t ->
+      bytes_to_token (token_to_bytes t ++ rest)
+                     (match t with Lit _ => true | Ref _ _ => false end) = (Some t, rest).
+    Proof.
+      intros.
+      destruct t.
+      - reflexivity.
+      - apply pair_equal_spec.
+        split; [f_equal | reflexivity].
+        f_equal.
+        + simpl in *.
+          pose proof (Nat.divmod_spec (offset - 3) 255 0 255 ltac:(lia)).
+          destruct (Nat.divmod (offset - 3) 255 0 255) as [q'1 u'1]. simpl.
+          rewrite (to_nat_nibbles_correct (length - 3) q'1 ltac:(lia) ltac:(lia)).
+          pose proof (Nat.divmod_spec ((length - 3) * 16 + q'1) 15 0 15 ltac:(lia)).
+          destruct (Nat.divmod ((length - 3) * 16 + q'1) 15 0 15) as [q'2 u'2]. simpl.
+          lia.
+        + unfold nibbles_to_byte.
+          pose proof (Nat.mod_upper_bound (offset - 3) 256 ltac:(lia)).
+          rewrite (nat_to_byte_correctness ((offset - 3) mod 256) ltac:(lia)).
+          assert ((length - 3) mod 16 * 16 + ((offset - 3) / 256) mod 16 < 256). {
+            pose proof (Nat.mod_upper_bound (length - 3) 16 ltac:(lia)).
+            pose proof (Nat.mod_upper_bound ((offset - 3) / 256) 16 ltac:(lia)).
+            lia.
+          }
+          rewrite (nat_to_byte_correctness ((length - 3) mod 16 * 16 + ((offset - 3) / 256) mod 16) H1).
+          unfold Nat.modulo, Nat.div.
+          pose proof (Nat.divmod_spec (length - 3) 15 0 15 ltac:(lia)).
+          destruct (Nat.divmod (length - 3) 15 0 15) as [q1 u1].
+          pose proof (Nat.divmod_spec (offset - 3) 255 0 255 ltac:(lia)).
+          destruct (Nat.divmod (offset - 3) 255 0 255) as [q2 u2].
+          assert (snd (q1, u1) = u1) by reflexivity.
+          rewrite H4. clear H4.
+          assert (snd (q2, u2) = u2) by reflexivity.
+          rewrite H4. clear H4.
+          assert (fst (q2, u2) = q2) by reflexivity.
+          rewrite H4. clear H4.
+          pose proof (Nat.divmod_spec q2 15 0 15 ltac:(lia)).
+          destruct (Nat.divmod q2 15 0 15) as [q3 u3].
+          assert (snd (q3, u3) = u3) by reflexivity.
+          rewrite H5. clear H5.
+          pose proof (Nat.divmod_spec ((15 - u1) * 16 + (15 - u3)) 15 0 15 ltac:(lia)).
+          destruct (Nat.divmod ((15 - u1) * 16 + (15 - u3)) 15 0 15) as [q4 u4].
+          assert (snd (q4, u4) = u4) by reflexivity.
+          rewrite H6. clear H6.
+          destruct H. lia.
+    Qed.
+
+    Lemma chunk_remove: forall n tokens acc flag_byte tail,
+      n <= 8 ->
+      Forall valid_token tokens ->
+      tokens_to_bytes_chunk n tokens = (flag_byte, tail, acc) ->
+      exists prev,
+        tokens = prev ++ tail /\
+        Forall valid_token prev /\
+        length prev = Nat.min n (length tokens) /\
+        tokens_to_bytes_chunk n prev = (flag_byte, [], acc).
+    Proof.
+      induction n; intros; simpl in H1.
+      - exists [].
+        repeat split; simpl.
+        + congruence.
+        + constructor.
+        + congruence.
+      - destruct tokens.
+        + exists [].
+          repeat split.
+          * inversion H1; subst. reflexivity.
+          * constructor.
+          * simpl. congruence.
+        + destruct (tokens_to_bytes_chunk n tokens) as [[b tail'] acc'] eqn:?.
+          destruct t.
+          * assert (true :: b = flag_byte) by congruence. subst.
+            assert (tail = tail') by congruence. subst.
+            assert (token_to_bytes (Lit b0) ++ acc' = acc) by congruence. subst.
+            inversion H0; subst.
+            specialize (IHn tokens acc' b tail' ltac:(lia) H5 Heqp).
+            destruct IHn as [prev [Heq [Hfa [Hlen Hp]]]].
+            exists (Lit b0 :: prev).
+            repeat split.
+            -- rewrite Heq. reflexivity.
+            -- constructor; assumption.
+            -- simpl. f_equal. assumption.
+            -- simpl. rewrite Hp. reflexivity.
+          * assert (false :: b = flag_byte) by congruence. subst.
+            assert (tail = tail') by congruence. subst.
+            assert (token_to_bytes (Ref length offset) ++ acc' = acc) by congruence. subst.
+            inversion H0; subst.
+            specialize (IHn tokens acc' b tail' ltac:(lia) H5 Heqp).
+            destruct IHn as [prev [Heq [Hfa [Hlen Hp]]]].
+            exists (Ref length offset :: prev).
+            repeat split.
+            -- rewrite Heq. reflexivity.
+            -- constructor; assumption.
+            -- simpl. f_equal. assumption.
+            -- simpl. rewrite Hp. reflexivity.
+    Qed.
+
+    Lemma bytes_to_token_app: forall flag acc rest token tail,
+      bytes_to_token acc flag = (Some token, tail) ->
+      bytes_to_token (acc ++ rest) flag = (Some token, tail ++ rest).
+    Proof.
+      intros. destruct flag, acc as [| b [| b0 tailB]];
+      simpl in H; try discriminate; injection H as <- <-; reflexivity.
+    Qed.
+
+    Lemma chunk_app: forall n flag acc rest tokens tail,
+      bytes_to_tokens_chunk n flag acc = (tokens, tail) ->
+      length tokens = n \/ rest = [] ->
+      bytes_to_tokens_chunk n flag (acc ++ rest) = (tokens, tail ++ rest).
+    Proof.
+      induction n; intros.
+      - simpl in *. congruence.
+      - simpl in H.
+        destruct (bytes_to_token acc (Nat.testbit flag n)) as [otoken tailB] eqn:?, otoken.
+        + destruct (bytes_to_tokens_chunk n flag tailB) as [tokensB restB] eqn:?.
+          injection H as <- <-.
+          simpl in H0 |- *. destruct H0.
+          * injection H as H.
+            rewrite (bytes_to_token_app (Nat.testbit flag n) acc rest t tailB Heqp).
+            rewrite (IHn flag tailB rest tokensB restB Heqp0); auto.
+          * subst.
+            repeat rewrite app_nil_r.
+            rewrite Heqp, Heqp0. reflexivity.
+        + injection H as <- <-.
+          simpl in H0. destruct H0.
+          * discriminate.
+          * subst. simpl.
+            repeat rewrite app_nil_r.
+            rewrite Heqp. reflexivity.
+    Qed.
+
+    Lemma tokens_to_bytes_chunk_flag_length: forall n tokens ts acc flag,
+      tokens_to_bytes_chunk n tokens = (flag, ts, acc) ->
+      length flag <= n.
+    Proof.
+      induction n; simpl; intros.
+      - inversion H; subst. now simpl.
+      - destruct tokens.
+        + inversion H; subst. simpl. lia.
+        + destruct (tokens_to_bytes_chunk n tokens) as [[flag' ts'] acc'] eqn:?.
+          inversion H. subst. simpl.
+          specialize (IHn tokens ts acc' flag' Heqp).
+          lia.
+    Qed.
+
+    Lemma zero_lt_2_pow: forall n,
+      0 < 2 ^ n.
+    Proof. intros. assert (2 ^ n <> 0) by (apply Nat.pow_nonzero; lia). lia. Qed.
+
+    Lemma list_bool_to_byte_correctness: forall l n x,
+      length l <= n ->
+      n <= 8 ->
+      x < 2 ^ (8 - n) ->
+      exists rest,
+        rest < 2 ^ n /\
+        to_nat (list_bool_to_byte l x n) = x * 2 ^ n + rest.
+    Proof.
+      induction l; intros; simpl.
+      - rewrite nat_to_byte_correctness.
+        + exists 0.
+          split.
+          * apply zero_lt_2_pow.
+          * lia.
+        + assert (x * 2 ^ n < 2 ^ (8 - n) * 2 ^ n). {
+            apply Nat.mul_lt_mono_pos_r.
+            - apply zero_lt_2_pow.
+            - assumption.
+          }
+          assert (8 - n + n = 8) by lia.
+          assert (1 * 2 ^ 8 = 256) by reflexivity.
+          rewrite <- 2 Nat.shiftl_mul_pow2, <- Nat.shiftl_1_l, Nat.shiftl_shiftl, H3,
+                  2 Nat.shiftl_mul_pow2 in H2.
+          now rewrite H4 in H2.
+      - destruct n.
+        + exists 0; simpl.
+          split.
+          * lia.
+          * rewrite nat_to_byte_correctness.
+            -- lia.
+            -- assert (2 ^ (8 - 0) = 256) by reflexivity. lia.
+        + assert (x * 2 + (if a then 1 else 0) < 2 ^ (8 - n)). {
+            replace (8 - S n) with (7 - n) in * by reflexivity.
+            rewrite Nat.mul_comm.
+            destruct a.
+            - clear l IHl H.
+              replace (8 - n) with (S (7 - n)) by lia.
+              change (2 ^ S (7 - n)) with (2 * (2 ^ (7 - n))).
+              lia.
+            - replace (2 ^ (8 - n)) with (2 * 2 ^ (7 - n)).
+              + lia.
+              + rewrite <- Nat.pow_succ_r'.
+                f_equal. lia.
+          }
+          destruct a.
+          * destruct (IHl n (x * 2 + 1) ltac:(simpl in H; lia) ltac:(lia) H2) as [rest [Hb Heq]].
+            exists (2 ^ n + rest).
+            split.
+            -- simpl. lia.
+            -- rewrite Heq. simpl. lia.
+          * destruct (IHl n (x * 2 + 0) ltac:(simpl in H; lia) ltac:(lia) H2) as [rest [Hb Heq]].
+            exists rest.
+            split.
+            -- simpl. lia.
+            -- rewrite Heq. simpl. lia.
+    Qed.
+
+    Lemma div_double_plus_r: forall n r,
+      Nat.div2 (2 * n + r) = n + Nat.div2 r.
+    Proof.
+      intros.
+      rewrite 2 Nat.div2_div. simpl.
+      pose proof (Nat.divmod_spec (n + (n + 0) + r) 1 0 1 ltac:(lia)).
+      destruct (Nat.divmod (n + (n + 0) + r) 1 0 1) as [q u].
+      pose proof (Nat.divmod_spec r 1 0 1 ltac:(lia)).
+      destruct (Nat.divmod r 1 0 1) as [q' u'].
+      simpl. lia.
+    Qed.
+
+    Lemma testbit_flag: forall b: bool, forall x rest n,
+      rest < 2 ^ n ->
+      Nat.testbit ((x * 2 + (if b then 1 else 0)) * 2 ^ n + rest) n = b.
+    Proof.
+      intros.
+      revert b x rest H.
+      induction n; simpl in *; intros.
+      - replace rest with 0 by lia.
+        rewrite Nat.add_0_r, Nat.mul_1_r, Nat.mul_comm.
+        destruct b.
+        + apply Nat.odd_odd.
+        + rewrite Nat.add_0_r. apply Nat.odd_even.
+      - assert (Nat.div2 rest < 2 ^ n). {
+          rewrite Nat.div2_div.
+          now apply Nat.Div0.div_lt_upper_bound.
+        }
+        replace (2 ^ n + (2 ^ n + 0)) with (2 * 2 ^ n) in * by reflexivity.
+        specialize (IHn b x (Nat.div2 rest) H0). simpl in IHn.
+        now rewrite Nat.mul_comm, <- Nat.mul_assoc, div_double_plus_r, Nat.mul_comm.
+    Qed.
+
+    Lemma to_tokens_chunk_correctness: forall n tokens acc flag_byte x,
+      n <= 8 ->
+      x < 2 ^ (8 - n) ->
+      Forall valid_token tokens ->
+      length tokens <= n ->
+      tokens_to_bytes_chunk n tokens = (flag_byte, [], acc) ->
+      bytes_to_tokens_chunk n (to_nat (list_bool_to_byte flag_byte x n)) acc = (tokens, []).
+    Proof.
+      induction n; intros; simpl in H3 |- *.
+      - congruence.
+      - destruct tokens.
+        + inversion H3; subst.
+          simpl bytes_to_tokens_chunk.
+          destruct (Nat.testbit (to_nat (list_bool_to_byte [] x (S n))) n); reflexivity.
+        + destruct (tokens_to_bytes_chunk n tokens) as [[flag ts'] acc'] eqn:?.
+          inversion H3. subst. clear H3.
+          set (b := match t with Lit _ => true | Ref _ _ => false end).
+          assert (to_nat (list_bool_to_byte flag (x * 2 + (if b then 1 else 0)) n) =
+                  to_nat (list_bool_to_byte (b :: flag) x (S n))) by reflexivity.
+          rewrite <- H3. clear H3.
+
+          assert (Hb: x * 2 + (if b then 1 else 0) < 2 ^ (8 - n)). {
+            assert (2 ^ (8 - n) = 2 ^ (8 - S n) * 2). {
+              replace (8 - n) with (S (8 - S n)) by lia.
+              rewrite Nat.pow_succ_r'. lia.
+            }
+            destruct b; lia.
+          }
+          pose proof (tokens_to_bytes_chunk_flag_length n tokens [] acc' flag Heqp).
+          pose proof (list_bool_to_byte_correctness flag n (x * 2 + (if b then 1 else 0)) H3
+                      ltac:(lia) Hb) as [rest [Hrb Heq]].
+          rewrite Heq.
+          rewrite testbit_flag by assumption.
+          inversion H1; subst.
+          rewrite to_token_correctness by assumption.
+          specialize (IHn tokens acc' flag (x * 2 + (if b then 1 else 0)) ltac:(lia) Hb H7
+                      ltac:(simpl in H2; lia) Heqp).
+          rewrite Heq in IHn.
+          now rewrite IHn.
+    Qed.
+
+    Lemma to_tokens_fueled_correctness: forall fuel1 fuel2 t l,
+      Forall valid_token t ->
+      length t <= fuel1 ->
+      tokens_to_bytes_fueled t fuel1 = l ->
+      length l <= fuel2 ->
+      bytes_to_tokens_fueled l fuel2 = t.
+    Proof.
+      induction fuel1; intros.
+      - inversion H0. apply length_zero_iff_nil in H4. subst.
+        destruct fuel2; reflexivity.
+      - destruct t.
+        + simpl in H1; subst. destruct fuel2; reflexivity.
+        + unfold tokens_to_bytes_fueled in H1.
+          destruct (tokens_to_bytes_chunk _ _) as [[flag restT] bytes] eqn:?.
+          match goal with
+          | [ H: _ :: _ ++ ?f _ _ = _ |- _ ] =>
+              assert (Hfun: f = tokens_to_bytes_fueled) by reflexivity; rewrite Hfun in H; clear Hfun
+          end.
+
+          unfold bytes_to_tokens_fueled.
+          destruct fuel2.
+          * inversion H2. apply length_zero_iff_nil in H4. subst. discriminate.
+          * destruct l. discriminate.
+            destruct (bytes_to_tokens_chunk 8 (to_nat b) l) as [tokens tail] eqn:?.
+            match goal with
+            | [ |- _ ++ ?f _ _ = _] =>
+                assert (Hfun: f = bytes_to_tokens_fueled) by reflexivity; rewrite Hfun; clear Hfun
+            end.
+
+            assert (list_bool_to_byte flag 0 8 = b) by congruence. subst.
+            injection H1 as H1.
+            pose proof (chunk_remove 8 (t :: t0) bytes flag restT ltac:(lia) H Heqp)
+                        as [prev [Heqpv [Hf [Hl Ht]]]].
+            pose proof (to_tokens_chunk_correctness 8 prev bytes flag 0 ltac:(lia)
+                        ltac:(apply zero_lt_2_pow) Hf ltac:(lia) Ht).
+            assert (Hor: length prev = 8 \/ tokens_to_bytes_fueled restT fuel1 = []). {
+              destruct (Nat.min_dec 8 (length (t :: t0))).
+              - left. lia.
+              - right.
+                assert (restT = []). {
+                  rewrite Heqpv, length_app, Hl in H0.
+                  destruct restT.
+                  - reflexivity.
+                  - rewrite e, Heqpv, length_app in Hl. simpl in Hl. lia.
+                }
+                subst. destruct fuel1; reflexivity.
+            }
+            pose proof (chunk_app 8 (to_nat (list_bool_to_byte flag 0 8)) bytes
+                        (tokens_to_bytes_fueled restT fuel1) prev [] H3 Hor).
+            rewrite app_nil_l in H4.
+            assert (prev = tokens) by congruence. subst.
+            rewrite Heqpv, app_inv_head_iff.
+            assert (Forall valid_token restT). {
+              rewrite Heqpv in H.
+              apply Forall_app in H. tauto.
+            }
+            assert (length restT <= fuel1). {
+              rewrite Heqpv in H0. simpl in H0.
+              rewrite length_app, Hl in H0.
+              simpl in H0. lia.
+            }
+            assert (length tail <= fuel2). {
+              assert (tail = tokens_to_bytes_fueled restT fuel1) by congruence. subst.
+              simpl in H2. rewrite length_app in H2.
+              lia.
+            }
+            exact (IHfuel1 fuel2 restT tail H1 H5 ltac:(congruence) H6).
+    Qed.
+
+    Theorem to_tokens_correctness: forall t,
+      Forall valid_token t ->
+      bytes_to_tokens (tokens_to_bytes t) = t.
+    Proof.
+      intros.
+      unfold bytes_to_tokens, tokens_to_bytes.
+      eapply to_tokens_fueled_correctness; trivial.
+    Qed.
+
+    Definition token_weight t :=
+      match t with
+      | Lit _ => 1
+      | Ref _ _ => 3
+      end.
+
+    Lemma chunk_length_bound': forall n seq,
+      n <= 8 ->
+      (tokens_to_bytes_chunk_len n seq) <= ((list_sum (map token_weight seq))).
+    Proof.
+      induction n; intros; destruct seq; simpl; try lia.
+      specialize (IHn seq ltac:(lia)).
+      destruct t; simpl; lia.
+    Qed.
+
+    Lemma chunk_length_bound: forall tokens n acc flag_byte tail,
+      n <= 8 ->
+      Forall valid_token tokens ->
+      tokens_to_bytes_chunk n tokens = (flag_byte, tail, acc) ->
+      exists prev,
+        tokens = prev ++ tail /\
+        (tail = [] \/ length prev = n) /\
+        length acc <= (list_sum (map token_weight prev)).
+    Proof.
+      intros.
+      pose proof (chunk_remove n tokens acc flag_byte tail H H0 H1).
+      destruct H2 as [prev [He [Hv [Hl Ht]]]].
+      exists prev.
+      repeat split.
+      - assumption.
+      - destruct tail.
+        + left. reflexivity.
+        + right. rewrite He, length_app in Hl.
+          simpl in Hl. lia.
+      - pose proof (chunk_length_bound' n prev H).
+        now rewrite <- (tokens_to_bytes_chunk_len_correctness n prev flag_byte [] acc Ht).
+    Qed.
+
+    Lemma tokens_to_bytes_bounded_by_weight : forall fuel tokens,
+      Forall valid_token tokens ->
+      length tokens <= fuel ->
+      length (tokens_to_bytes_fueled tokens fuel) <= ((9 * (list_sum (map token_weight tokens))) + 7) / 8.
+    Proof.
+      induction fuel; intros.
+      - simpl. lia.
+      - destruct tokens.
+        + simpl. lia.
+        + unfold tokens_to_bytes_fueled.
+          destruct (tokens_to_bytes_chunk 8 (t :: tokens)) as [[flag tail] acc] eqn:?.
+          simpl length. rewrite length_app.
+          destruct (chunk_length_bound (t :: tokens) 8 acc flag tail ltac:(lia) H Heqp)
+                    as (prev & Ht & Hor & Hl).
+          simpl in H.
+          match goal with
+          | [ |- context[length (?fn ?t ?f)] ] =>
+              assert (He: fn t f = tokens_to_bytes_fueled tail fuel)
+                      by reflexivity; rewrite He; clear He
+          end.
+          assert (Hlf: length tail <= fuel). {
+            apply le_S_n in H0.
+            destruct prev.
+            - simpl in Hl. inversion Hl. apply length_zero_iff_nil in H2.
+              simpl in Ht. subst.
+              simpl in Heqp.
+              do 8 (destruct tokens; simpl in Heqp; try discriminate).
+              destruct t, t0, t1, t2, t3, t4, t5, t6, t7; discriminate.
+            - simpl in Ht.
+              assert (tokens = prev ++ tail) by congruence.
+              rewrite H1 in H0.
+              match goal with
+              | [ H: context[?fn (prev ++ tail)] |- _ ] =>
+                  assert (Hfn: fn (prev ++ tail) = length (prev ++ tail))
+                          by reflexivity; rewrite Hfn in H; clear Hfn
+              end.
+              rewrite length_app in H0. lia.
+          }
+          rewrite Ht in H.
+          destruct (Forall_app valid_token prev tail) as [H1 _].
+          destruct (H1 H) as [_ H2].
+          specialize (IHfuel tail H2 Hlf).
+          rewrite Ht, map_app, list_sum_app.
+          eapply Nat.le_trans with (m :=
+                 S (list_sum (map token_weight prev) + (9 * list_sum (map token_weight tail) + 7) / 8)).
+          * lia.
+          * assert (prev <> []). {
+              destruct prev.
+              - simpl in Hl. inversion Hl. apply length_zero_iff_nil in H4.
+                simpl in Ht. subst.
+                simpl in Heqp.
+                do 8 (destruct tokens; simpl in Heqp; try discriminate).
+                destruct t, t0, t1, t2, t3, t4, t5, t6, t7; discriminate.
+              - discriminate.
+            }
+            set (x := list_sum (map token_weight prev)).
+            set (y := list_sum (map token_weight tail)).
+            destruct Hor.
+            -- assert (1 <= x). {
+                 destruct prev.
+                 - contradiction.
+                 - simpl in x. destruct t0; simpl in x; lia.
+               }
+               subst. simpl in y |- *.
+               match goal with
+               | [ |- context[Nat.divmod ?x ?y ?q ?u] ] =>
+                   pose proof (Nat.divmod_spec x y q u ltac:(lia));
+                   destruct (Nat.divmod x y q u) eqn:?
+               end.
+               simpl. lia.
+            -- assert (8 <= x). {
+                 do 8 (destruct prev; try (simpl in H4; lia)).
+                 destruct t0, t1, t2, t3, t4, t5, t6, t7; simpl in x; lia.
+               }
+               simpl.
+               do 2 match goal with
+               | [ |- context[Nat.divmod ?x ?y ?q ?u] ] =>
+                   pose proof (Nat.divmod_spec x y q u ltac:(lia));
+                   destruct (Nat.divmod x y q u) eqn:?
+               end.
+               simpl. lia.
+    Qed.
+  End TokenBytes.
+
+End Tokens.
+
+Export Tokens.
